Reorganize and start adding comments.

theories/unsafe.v
@@ -1,46 +1,169 @@
 From tutorial_popl20 Require Export sem_typing.
-From iris.heap_lang.lib Require Import assert.
-From tutorial_popl20 Require Export symbol_ghost.
+From tutorial_popl20 Require Import symbol_ghost two_state_ghost.
 
-(* Semantic typing of a symbol ADT (taken from Dreyer's POPL'18 talk) *)
-Definition symbol_adt_inc : val := λ: "x" <>, FAA "x" #1.
-Definition symbol_adt_check : val := λ: "x" "y", assert: "y" < !"x".
-Definition symbol_adt : val := λ: <>,
-  let: "x" := Alloc #0 in (symbol_adt_inc "x", symbol_adt_check "x").
+Section unsafe.
+  Context `{heapG Σ}.
 
-Definition symbol_adt_ty `{heapG Σ} : sem_ty Σ :=
-  (() → ∃ A, (() → A) * (A → ()))%sem_ty.
+  (** * Exercise (easy) *)
+  Definition unsafe_pure : val := λ: <>,
+    if: #true then #13 else #13 #37.
 
-Section sem_typed_symbol_adt.
-  Context `{heapG Σ, symbolG Σ}.
-
-  Definition symbol_adtN := nroot .@ "symbol_adt".
-
-  Definition symbol_inv (γ : gname) (l : loc) : iProp Σ :=
-    (∃ n : nat, l ↦ #n ∗ counter γ n)%I.
-
-  Definition sem_ty_symbol (γ : gname) : sem_ty Σ := SemTy (λ w,
-    ∃ n : nat, ⌜w = #n⌝ ∧ symbol γ n)%I.
-
-  Lemma sem_typed_symbol_adt Γ : Γ ⊨ symbol_adt : symbol_adt_ty.
+  Lemma sem_typed_unsafe_pure : ∅ ⊨ unsafe_pure : () → sem_ty_int.
   Proof.
-    iIntros (vs) "!# _ /=". iApply wp_value.
-    iIntros "!#" (v ->). wp_lam. wp_alloc l as "Hl"; wp_pures.
-    iMod (counter_alloc 0) as (γ) "Hc".
-    iMod (inv_alloc symbol_adtN _ (symbol_inv γ l) with "[Hl Hc]") as "#?".
-    { iExists 0%nat. by iFrame. }
-    do 2 (wp_lam; wp_pures).
-    iExists (sem_ty_symbol γ), _, _; repeat iSplit=> //.
-    - repeat rewrite /sem_ty_car /=. iIntros "!#" (? ->). wp_pures.
-      iInv symbol_adtN as (n) ">[Hl Hc]". wp_faa.
-      iMod (counter_inc with "Hc") as "[Hc #Hs]".
-      iModIntro; iSplitL; last eauto.
-      iExists (S n). rewrite Nat2Z.inj_succ -Z.add_1_r. iFrame.
-    - repeat rewrite /sem_ty_car /=. iIntros "!#" (v).
-      iDestruct 1 as (n ->) "#Hs". wp_pures. iApply wp_assert.
-      wp_bind (!_)%E. iInv symbol_adtN as (n') ">[Hl Hc]". wp_load.
-      iDestruct (symbol_obs with "Hc Hs") as %?. iModIntro. iSplitL.
-      { iExists n'. iFrame. }
-      wp_op. rewrite bool_decide_true; last lia. eauto.
+    iIntros (vs) "!# HΓ"; simpl.
+    iApply wp_value.
+    iIntros "!#" (? ->).
+    wp_lam.
+    wp_if.
+    rewrite /sem_ty_car /=.
+    by iExists 13.
   Qed.
-End sem_typed_symbol_adt.
+
+  (** * Exercise (easy) *)
+  Definition unsafe_ref : val := λ: <>,
+    let: "l" := ref #0 in "l" <- #true;; !"l".
+
+  Lemma sem_typed_unsafe_ref : ∅ ⊨ unsafe_ref : () → sem_ty_bool.
+  Proof.
+    iIntros (vs) "!# HΓ"; simpl.
+    iApply wp_value.
+    iIntros "!#" (? ->).
+    wp_lam.
+    wp_alloc l as "Hl".
+    wp_let.
+    wp_store.
+    wp_load.
+    rewrite /sem_ty_car /=.
+    by iExists true.
+  Qed.
+
+  (** * Exercise (moderate) *)
+  Definition unsafe_ref_ne_0 : val := λ: <>,
+    let: "l" := ref #1 in
+    ((λ: "x", if: "x" ≠ #0 then "l" <- "x" else #()),
+     (λ: <>, assert: !"l" ≠ #0)).
+
+  Lemma sem_typed_unsafe_ref_ne_0 :
+    ∅ ⊨ unsafe_ref_ne_0 : () → (sem_ty_int → ()) * (() → ()).
+  Proof.
+    iIntros (vs) "!# HΓ"; simpl.
+    iApply wp_value.
+    iIntros "!#" (? ->).
+    wp_lam.
+    wp_alloc l as "Hl".
+    wp_let.
+    pose (I := (∃ n : Z, ⌜#n ≠ #0⌝ ∗ l ↦ #n)%I).
+    iMod (inv_alloc (nroot .@ "exercise3") _ I with "[Hl]")%I as "#Hinv".
+    { by iNext; iExists 1; iFrame. }
+    wp_pures.
+    iExists _, _. iSplit; first done.
+    iSplit.
+    - iIntros "!#" (? [n ->]).
+      wp_lam.
+      wp_op.
+      destruct (decide (n = 0%Z)); simplify_eq/=.
+      + wp_op.
+        wp_if.
+        done.
+      + rewrite bool_decide_eq_false_2; last congruence.
+        wp_op.
+        wp_if.
+        iInv (nroot .@ "exercise3") as (m) ">[% Hl]".
+        wp_store.
+        iModIntro. iSplit.
+        * iExists n; auto with congruence.
+        * done.
+    - iIntros "!#" (? ->).
+      wp_lam.
+      wp_pures.
+      iApply wp_assert.
+      (* Need because of atomic expression *)
+      wp_bind (! _)%E.
+      iInv (nroot .@ "exercise3") as (m) ">[% Hl]".
+      wp_load.
+      iModIntro. iSplitL "Hl".
+      { iExists m; auto. }
+      wp_op.
+      rewrite bool_decide_eq_false_2; last done.
+      by wp_op.
+  Qed.
+
+  (** * Exercise (hard) *)
+  Definition unsafe_ref_reuse : val :=
+    λ: <>, let: "l" := ref #0 in λ: <>, "l" <- #true;; !"l".
+
+  Lemma sem_typed_unsafe_ref_reuse `{two_stateG Σ}:
+    ∅ ⊨ unsafe_ref_reuse : () → (() → sem_ty_bool).
+  Proof.
+    iIntros (vs) "!# HΓ"; simpl.
+    iApply wp_value.
+    iIntros "!#" (? ->).
+    wp_lam.
+    wp_alloc l as "Hl".
+    iMod two_state_init as (γ) "Ho".
+    pose (I := (∃ b, two_state_auth γ b ∗ l ↦ (if b then #true else #0))%I).
+    iMod (inv_alloc (nroot .@ "exercise4") _ I with "[Hl Ho]") as "#Hinv".
+    { iNext. iExists false. iFrame. }
+    wp_pures.
+    iIntros "!#" (? ->).
+    wp_lam.
+    (* Need because of atomic expression *)
+    wp_bind (_ <- _)%E.
+    iInv (nroot .@ "exercise4") as (o) ">[Ho Hl]".
+    wp_store.
+    iMod (two_state_update with "Ho") as "[Ho Hf]".
+    iModIntro. iSplitL "Hl Ho".
+    { iNext. iExists true. iFrame. }
+    wp_pures.
+    iInv (nroot .@ "exercise4") as (o') ">[Ho Hl]".
+    iDestruct (two_state_agree with "Ho Hf") as %->.
+    wp_load.
+    iModIntro. iSplitL "Hl Ho".
+    { iNext. iExists true. iFrame. }
+    rewrite /sem_ty_car /=. by iExists _.
+  Qed.
+
+  (** * Exercise (hard) *)
+  (** Semantic typing of a symbol ADT (taken from Dreyer's POPL'18 talk) *)
+  Definition symbol_adt_inc : val := λ: "x" <>, FAA "x" #1.
+  Definition symbol_adt_check : val := λ: "x" "y", assert: "y" < !"x".
+  Definition symbol_adt : val := λ: <>,
+    let: "x" := Alloc #0 in (symbol_adt_inc "x", symbol_adt_check "x").
+
+  Definition symbol_adt_ty `{heapG Σ} : sem_ty Σ :=
+    (() → ∃ A, (() → A) * (A → ())).
+
+  Section sem_typed_symbol_adt.
+    Context `{heapG Σ, symbolG Σ}.
+
+    Definition symbol_adtN := nroot .@ "symbol_adt".
+
+    Definition symbol_inv (γ : gname) (l : loc) : iProp Σ :=
+      (∃ n : nat, l ↦ #n ∗ counter γ n)%I.
+
+    Definition sem_ty_symbol (γ : gname) : sem_ty Σ := SemTy (λ w,
+      ∃ n : nat, ⌜w = #n⌝ ∧ symbol γ n)%I.
+
+    Lemma sem_typed_symbol_adt Γ : Γ ⊨ symbol_adt : symbol_adt_ty.
+    Proof.
+      iIntros (vs) "!# _ /=". iApply wp_value.
+      iIntros "!#" (v ->). wp_lam. wp_alloc l as "Hl"; wp_pures.
+      iMod (counter_alloc 0) as (γ) "Hc".
+      iMod (inv_alloc symbol_adtN _ (symbol_inv γ l) with "[Hl Hc]") as "#?".
+      { iExists 0%nat. by iFrame. }
+      do 2 (wp_lam; wp_pures).
+      iExists (sem_ty_symbol γ), _, _; repeat iSplit=> //.
+      - repeat rewrite /sem_ty_car /=. iIntros "!#" (? ->). wp_pures.
+        iInv symbol_adtN as (n) ">[Hl Hc]". wp_faa.
+        iMod (counter_inc with "Hc") as "[Hc #Hs]".
+        iModIntro; iSplitL; last eauto.
+        iExists (S n). rewrite Nat2Z.inj_succ -Z.add_1_r. iFrame.
+      - repeat rewrite /sem_ty_car /=. iIntros "!#" (v).
+        iDestruct 1 as (n ->) "#Hs". wp_pures. iApply wp_assert.
+        wp_bind (!_)%E. iInv symbol_adtN as (n') ">[Hl Hc]". wp_load.
+        iDestruct (symbol_obs with "Hc Hs") as %?. iModIntro. iSplitL.
+        { iExists n'. iFrame. }
+        wp_op. rewrite bool_decide_true; last lia. eauto.
+    Qed.
+  End sem_typed_symbol_adt.
+End unsafe.
