theories/parametricity.v
@@ -1,0 +1,24 @@
+From tutorial_popl20 Require Export safety.
+
+Section parametricity.
+  Context `{heapG Σ}.
+
+  (* REMOVE *) Definition exercise5_sem_ty Σ (v : val) : sem_ty Σ :=
+    SemTy (λ w, ⌜w = v⌝)%I.
+
+  Lemma exercise5 `{!heapPreG Σ} e (v : val) σ w es σ' :
+    (∀ `{heapG Σ}, ∅ ⊨ e : ∀ A, A → A) →
+    rtc erased_step ([e ! v]%E, σ) (of_val w :: es, σ') → w = v.
+  (* REMOVE *) Proof.
+    intros He.
+    apply sem_gen_type_safety with (φ := λ u, u = v)=> ?.
+    exists (exercise5_sem_ty Σ v). split.
+    { by iIntros (?) "?". }
+    iIntros (vs) "!# #Hvs".
+    iPoseProof (He with "Hvs") as "He /=".
+    wp_apply (wp_wand with "He").
+    iIntros (u) "#Hu".
+    iSpecialize ("Hu" $! (exercise5_sem_ty Σ v)).
+    wp_apply (wp_wand with "Hu"). iIntros (w') "Hw'". by iApply "Hw'".
+  Qed.
+End parametricity.
